theories/autosubst_preds.v
@@ -2,19 +2,67 @@ From Coq.ssr Require Import ssreflect.
 From stdpp Require Import base.
 From Autosubst Require Import Autosubst.
 
+(**
+    Goal: we want to be able to parameterize a datatype over an unspecified sort, and define
+    Autosubst 1 operations.
+
+    Substituting one sort through all the other sorts is not a usecase that Autosubst 1
+    was designed for, but it works. However, we end up needing a few extra lemmas about rename.
+
+    Here's the ones I needed in my proofs. *)
+Class HRenameLemmas (vl α: Type)
+  `{!Ids α} `{!Rename α}
+  `{!Ids vl} `{!Rename vl} `{!Subst vl} `{!HSubst vl α} := {
+  mixin_α_rename_Lemma :>
+    ∀ (ξ : var → var) (a : α), rename ξ a = a.|[ren ξ];
+  mixin_α_comp_rename_Lemma :>
+    ∀ (ξ : var → var) (σ : var → vl) (a: α),
+    (rename ξ a).|[σ] = a.|[ξ >>> σ];
+  mixin_α_rename_comp_Lemma :>
+    ∀ (σ : var → vl) (ξ : var → var) (t : α),
+    rename ξ t.|[σ] = t.|[σ >>> rename ξ];
+  mixin_α_comp_Lemma :>
+    ∀ (σ τ : var → vl) (t : α), t.|[σ].|[τ] = t.|[σ >> τ]
+}.
+
+Section HRenameLemmas.
+  Context `{RL: HRenameLemmas vl α}.
+
+  Lemma α_rename_Lemma: ∀ (ξ : var → var) (a : α), rename ξ a = a.|[ren ξ].
+  Proof. by destruct RL. Qed.
+
+  Lemma α_comp_rename_Lemma: ∀ (ξ : var → var) (σ : var → vl) (a: α),
+    (rename ξ a).|[σ] = a.|[ξ >>> σ].
+  Proof. by destruct RL. Qed.
+
+  Lemma α_rename_comp_Lemma: ∀ (σ : var → vl) (ξ : var → var) (t : α),
+    rename ξ t.|[σ] = t.|[σ >>> rename ξ].
+  Proof. by destruct RL. Qed.
+
+  Lemma α_comp_Lemma: ∀ (σ τ : var → vl) (t : α), t.|[σ].|[τ] = t.|[σ >> τ].
+  Proof. by destruct RL. Qed.
+End HRenameLemmas.
+
 Section composition.
-  Context (vl: Type) `{!Ids vl, !Rename vl, !Subst vl, SubstLemmas vl}.
+  Context (vl: Type) {Rename_vl: Rename vl} `{!Ids vl, !Subst vl, !SubstLemmas vl}.
 
   Definition pred := (var -> vl) → vl → Prop.
 
-  Instance HSubst_pred : HSubst vl pred := fun sb pred ρ => pred (sb >> ρ).
+  Global Instance Rename_pred : Rename pred := fun r pred ρ => pred (r >>> ρ).
 
-  Instance Rename_pred : Rename pred := fun r pred => pred.|[ren r].
-  Instance Inh_pred : Inhabited pred := populate (fun _ _ => False).
-  Instance Ids_pred : Ids pred := λ _, inhabitant.
+  Global Instance HSubst_pred : HSubst vl pred := fun sb pred ρ => pred (sb >> ρ).
 
-  Instance HSubstLemmas_pred : HSubstLemmas vl pred.
+  Global Instance Inh_pred : Inhabited pred := populate (fun _ _ => False).
+  Global Instance Ids_pred : Ids pred := λ _, inhabitant.
+
+  Global Instance HSubstLemmas_pred : HSubstLemmas vl pred.
   Proof.
     split; rewrite /hsubst /HSubst_pred => //= *; f_ext => ?; by asimpl.
+  Qed.
+
+  Global Instance HRenameLemmas_pred : HRenameLemmas vl pred.
+  Proof.
+    split; rewrite /rename /hsubst /Rename_pred /HSubst_pred //=; intros; f_ext => ?;
+      fold (@rename _ Rename_vl); by asimpl.
   Qed.
 End composition.
